knot/KnotMainIAproof.v
@@ -14,7 +14,7 @@ Module KnotMainIA. Section KnotMainIA.
   (* 1. global environment *)
   Context (genv: GEnv.t).
   (* 3. spec tables *)
-  Context (Sp: string -> option fspec).
+  Context (Sp: sp_type).
   Context (SpRec SpFun SpPure: spl_type).
   (* 4. hypotheses for genv *)
   Context (GEnvWF: GEnv.wf genv).
@@ -127,14 +127,16 @@ Module KnotMainIA. Section KnotMainIA.
     { (* prove the precondition of "fib" *)
       iFrame. iSplit; et. iPureIntro. eexists. esplits; et. econs; esplits; et.
       eapply fn_has_weaker_spec_in.
-      { econs; [|refl]. apply MainInFun. unfold MainFunSp. unseal CRIS. ss. }
+      { econs; [|instantiate (2:= Some (fspec_to_rel _)); s; refl].
+        apply MainInFun. unfold MainFunSp. unseal CRIS. ss. }
       { unfold fspec_imply, precond, postcond, fun_gen, fib_spec, fun_gen, fib_spec, fspec_apc; ss. 
-        ii. exists (x1, (knot_frag (Some Fib))%I). split; red.
+        ii. rr in ValidSP; des; subst. eexists _, _; split; [rr;et|].
+        instantiate (1:= (x, (knot_frag (Some Fib))%I)). split; red.
         { i. iIntros "[[% FG] %]". unfold precond, fun_gen, fib_spec; ss.
           des; subst; hss. iModIntro. iSplit; et. iSplit; et; cycle 1.
           iPureIntro. exists fb. esplits; et. inv H5. econs; et. eapply fn_has_weaker_spec_in; et.
           unfold fspec_imply, precond, postcond, fun_gen, fib_spec, fun_gen, fib_spec, fspec_apc; ss.
-          ii. eexists. split; red.
+          ii. rr in ValidSP; des; subst. eexists _, _; split; [rr; et|]. split; red.
           { red. instantiate (1:=(_, x0)). ss. iIntros; iFrame; et. }
           { i. ss. iIntros; et. }
         }
